added hw4 first work

hw4/testHW4.v
@@ -1,13 +1,111 @@
 Require Import Coq.Bool.Bool.
-Require Import Coq.Lists.List.
-Import ListNotations.
 
-Require Import Maps.
+Inductive bool_exp : Type :=
+  | BTrue : bool_exp
+  | BFalse : bool_exp
+  | BNot : bool_exp -> bool_exp
+  | BAnd : bool_exp -> bool_exp -> bool_exp
+  | BOr : bool_exp -> bool_exp -> bool_exp.
 
-Inductive bexp : Type :=
-  | BTrue : bexp
-  | BFalse : bexp
-  | BEq : aexp -> aexp -> bexp
-  | BLe : aexp -> aexp -> bexp
-  | BNot : bexp -> bexp
-  | BAnd : bexp -> bexp -> bexp.
+
+Fixpoint bool_eval (b : bool_exp) : bool :=
+  match b with
+  | BTrue       => true
+  | BFalse      => false
+  | BNot b1     => negb (bool_eval b1)
+  | BAnd b1 b2  => andb (bool_eval b1) (bool_eval b2)
+  | BOr b1 b2   => orb (bool_eval b1) (bool_eval b2)
+  end.
+
+Example test_bool_eval1:
+  bool_eval (BOr BTrue BFalse) = true.
+Proof. reflexivity. Qed.
+
+Example test_bool_eval2:
+  bool_eval (BAnd BTrue BFalse) = false.
+Proof. reflexivity. Qed.
+
+Example test_bool_eval3:
+  bool_eval (BNot BFalse) = true.
+Proof. reflexivity. Qed.
+
+Fixpoint simp_not (b:bool_exp) : bool_exp :=
+  match b with
+  | BTrue => BTrue
+  | BFalse => BFalse
+  | BNot b' => simp_not b'
+  | BOr b1 b2 => BOr (simp_not b1) (simp_not b2)
+  | BAnd b1 b2 => BAnd (simp_not b1) (simp_not b2)
+  end.
+
+Example test_simp_not1:
+  bool_eval (simp_not (BOr BTrue BFalse)) = true.
+Proof. simpl. reflexivity. Qed.
+
+
+Example test_simp_not2:
+  bool_eval (simp_not (BAnd (BNot BFalse) BFalse)) = false.
+Proof. simpl. reflexivity. Qed.
+
+
+Example test_simp_not3:
+  bool_eval (simp_not (BNot (BNot BTrue))) = true.
+Proof. simpl. reflexivity. Qed.
+
+Fixpoint simp_or (b:bool_exp) : bool_exp :=
+  match b with
+  | BTrue => BTrue
+  | BFalse => BFalse
+  | BNot b' => BNot (simp_or b')
+  | BOr BFalse b' => simp_or b'
+  | BOr b' BFalse => simp_or b'
+  | BOr b1 b2 => BOr (simp_or b1) (simp_or b2)
+  | BAnd b1 b2 => BAnd (simp_or b1) (simp_or b2)
+  end.
+
+Example test_simp_or1:
+  bool_eval (simp_or (BOr BTrue BFalse)) = true.
+Proof. simpl. reflexivity. Qed.
+
+Example test_simp_or2:
+  bool_eval (simp_or (BAnd (BNot BFalse) BFalse)) = false.
+Proof. simpl. reflexivity. Qed.
+
+Fixpoint simp_and (b:bool_exp) : bool_exp :=
+  match b with
+  | BTrue => BTrue
+  | BFalse => BFalse
+  | BNot b' => BNot (simp_and b')
+  | BAnd BTrue b' => simp_and b'
+  | BAnd b' BTrue => simp_and b'
+  | BAnd b1 b2 => BAnd (simp_and b1) (simp_and b2)
+  | BOr b1 b2 => BOr (simp_and b1) (simp_and b2)
+  end.
+
+Example test_simp_and1:
+  bool_eval (simp_and (BOr BTrue BFalse)) = true.
+Proof. simpl. reflexivity. Qed.
+
+Example test_simp_and2:
+  bool_eval (simp_and (BAnd (BNot BFalse) BFalse)) = false.
+Proof. simpl. reflexivity. Qed.
+
+Fixpoint simp_bool (b:bool_exp) : bool_exp :=
+  match b with 
+  | BTrue => BTrue
+  | BFalse => BFalse
+  | BNot b' => simp_not (simp_bool b')
+  | BOr b1 b2 => simp_or (BOr (simp_bool b1) (simp_bool b2))
+  | BAnd b1 b2 => simp_and (BAnd (simp_bool b1) (simp_bool b2))
+  end.
+
+Example test_simp_bool1:
+  bool_eval (simp_bool (BAnd (BNot BFalse) BFalse)) = false.
+Proof. simpl. reflexivity. Qed.
+
+Example test_simp_bool2:
+  bool_eval (simp_bool (BNot (BAnd BTrue BFalse))) = true.
+Proof. simpl. reflexivity. Qed.
+
+
+
